Snapshot

Allocator.lean
@@ -1,4 +1,4 @@
--- Linear Memory Allocation on a 16-bit memory space
+-- Linear Memory Allocation
 
 /-
 Note: many interesting properties that we could prove here:
@@ -11,7 +11,7 @@ Note: many interesting properties that we could prove here:
 
   - etc.
 -/
-
+open Classical
 
 abbrev Pointer := Nat
 
@@ -29,9 +29,12 @@ def Block.end (block : Block) : Pointer := block.ptr + block.size
 abbrev Blocks := List Block
 
 structure Allocator where
-  freeList : Blocks := [(0, 2^16)] -- sorted by first argument (ptr)
+  freeList : Blocks -- sorted by first argument (ptr)
   usedList : Blocks := [] -- could/should we use a HashMap instead?
 deriving Repr
+
+def Allocator.empty (size: Size) : Allocator :=
+  { freeList := if size == 0 then [] else [(0, size)] }
 
 -- The returned Nat refers the pointer.
 def Allocator.alloc₀ (allocator : Allocator) (size: Nat) : Option (Nat × Allocator) := do
@@ -67,7 +70,7 @@ def findBlock (size: Size) (done_todo : Blocks × Blocks) : Blocks × Blocks :=
     else
       findBlock size (done ++ [(ptr, currentSize)], rest)
   termination_by
-    done_todo.2.length -- That was surprisingly easy!
+    done_todo.2.length
 
 def Allocator.alloc₁ (allocator : Allocator) (size: Size) : Option (Pointer × Allocator) :=
   if size == 0 then
@@ -83,24 +86,27 @@ def Allocator.alloc₁ (allocator : Allocator) (size: Size) : Option (Pointer ×
       else
           [] -- perfect fit, remove the free block entirely
       let freeList := done ++ newFreeBlocks ++ rest
-      let usedList := (ptr, size) :: allocator.usedList
+      let usedList := allocator.usedList ++ [(ptr, size)]
       some (ptr, { allocator with freeList, usedList })
 
 def Allocator.alloc := Allocator.alloc₁
 
+-- TODO: split this test in several smaller ones.
 #eval do
-  let allocator : Allocator := {}
-  let (ptr₁, allocator) <- allocator.alloc 512
-  let (ptr₂, allocator) <- allocator.alloc 1024
-  let (ptr₃, allocator) <- allocator.alloc 0
-  let (ptr₄, allocator) <- allocator.alloc 1024
-  return ([ptr₁, ptr₂, ptr₃, ptr₄], allocator)
--- some (
---   [0, 512, 0, 1536],
---   {
---     freeList := [(2560, 62976)],
---     usedList := [(1536, 1024), (512, 1024), (0, 512)]
---   })
+  let allocator := Allocator.empty 8
+  let (_, allocator) <- allocator.alloc 0
+  let (ptr₁, allocator) <- allocator.alloc 1
+  let (ptr₂, allocator) <- allocator.alloc 2
+  let (_, allocator) <- allocator.alloc 0
+  let (ptr₃, allocator) <- allocator.alloc 3
+  return ([ptr₁, ptr₂, ptr₃], allocator)
+-- some ([0, 1, 3], { freeList := [(6, 2)], usedList := [(0, 1), (1, 2), (3, 3)] })
+
+#eval do
+  let allocator := Allocator.empty 8
+  let (ptr, allocator) <- allocator.alloc 9
+  return (ptr, allocator)
+-- none
 
 -- Step 2: Freeing memory
 partial def Allocator.free (allocator : Allocator) (ptr: Pointer) : Option Allocator := do
@@ -109,41 +115,99 @@ partial def Allocator.free (allocator : Allocator) (ptr: Pointer) : Option Alloc
   let block <- usedList.find? (·.1 == ptr)
   let usedList := usedList.filter (· != block)
   let freeList := (block :: freeList) |>.mergeSort (·.1 < ·.1)
-  return { allocator with freeList, usedList }.compact
+  return { allocator with freeList, usedList } -- no compaction yet
 
+-- TODO: (Arena-like properties) prove that:
+-- 0. 1 allocation of size 0 always succeeds (not matter what the state if the alloc is)
+-- 1. 1 allocation of total size <= available size (from empty) succeeds
+-- 2. several allocations of total size <= available size succeed
+-- 3. you can request largest spot and use it to guess if your alloc will
+--    succeed
+-- Other: show that for any sequence of non-zero allocs,
+-- all the pointers are distinct?
+
+theorem alloc_zero_succeeds : ∀ (allocator : Allocator), (allocator.alloc 0).isSome := by
+  simp [Allocator.alloc, Allocator.alloc₁]
+
+theorem alloc_one_succeeds_if_available :
+  ∀ (asked available : Size),
+  asked <= available ->
+  (Allocator.empty available |>.alloc asked |>.isSome) := by
+  intros asked available asked_le_available
+  simp [Allocator.alloc, Allocator.alloc₁]
+  -- TODO: cases on asked = 0 and asked > 0, simplify
+  cases (em (asked = 0)) with -- That's a hammer here.
+  | inl asked_zero => simp [asked_zero]
+  | inr asked_pos =>
+    simp [asked_pos]
+    simp [Allocator.empty]
+    cases (em (available = 0)) with
+    | inl available_eq_zero =>
+      rw [available_eq_zero] at asked_le_available
+      rw [Nat.le_zero] at asked_le_available
+      contradiction
+    | inr available_pos =>
+      simp [available_pos]
+      simp [findBlock]
+      simp [asked_le_available]
+
+/-
+Challenges for 2. :
+  - need a way to express chained allocations first
+  - proof uses structural induction on the list of sizes
+-/
+
+-- TODO: use mapM? declare the function as the appropriate StateT monad first?
+def Allocator.chainAlloc₀ (sizes : List Size) (allocator : Allocator) : Option (List Pointer × Allocator) := do
+  let mut pointers : List Pointer := []
+  let mut currentAllocator := allocator
+  for size in sizes do
+    match currentAllocator.alloc size with
+    | none => none -- failure
+    | some (pointer, newAllocator) =>
+      pointers := pointers ++ [pointer]
+      currentAllocator := newAllocator
+  return (pointers, currentAllocator)
+
+abbrev Allocation := StateT Allocator Option -- Any op that requires an alloc that may fail
+
+def Allocator.chainAlloc₁ (sizes : List Size) : Allocation (List Pointer) := do
+  let mut pointers : List Pointer := []
+  for size in sizes do
+    let allocation := (Allocator.alloc (size := size))
+    pointers := pointers ++ [<- allocation]
+  return pointers
+
+def Allocator.chainAlloc₂ (sizes : List Size) : Allocation (List Pointer) :=
+  let sizeToAlloc := fun (size : Size) => Allocator.alloc (size := size)
+  sizes.mapM sizeToAlloc
+
+def Allocator.chainAlloc := Allocator.chainAlloc₂
+
+theorem alloc_several_succeed_if_available :
+  ∀ (sizes : List Size), ∀ (available : Size),
+  sizes.sum <= available ->
+  (Allocator.empty available |>.chainAlloc sizes |>.isSome) := by
+  admit
+
+
+-- TODO: Beyond Arena : Freeing memory:
+-- 1. if you free some memory and allocate as many times 1 byte as needed,
+--    you end up using all this memory again (before you fail).
+--    More abstractly, show that there is a pattern of alloc that can use
+--    any byte in the region?
+
+#eval do
+  let allocator := Allocator.empty 8
+  let (ptr₁, allocator) <- allocator.alloc 1
+  let (ptr₂, allocator) <- allocator.alloc 2
+  let (_, allocator) <- allocator.alloc 3
+  let allocator <- allocator.free ptr₁
+  let allocator <- allocator.free ptr₂
+  return allocator
+-- some { freeList := [(0, 1), (1, 2), (6, 2)], usedList := [(3, 3)] }
 
 -- Later : reconsider "compaction" of free blocks.
-
--- -- Find the first free block in the memory large enough to contain the requested number of Bytes.
--- -- Return before, current and after blocks (maybe stupid, we could just do a List.find afterwards).
--- -- Dunno. Keep it like that ATM.
--- def Allocator.findFreeBlock (allocator : Allocator) (size: Size) : Option (Blocks × Block × Blocks) := do
---   let freeList := allocator.freeList
---   guard !freeList.isEmpty
---   let mut before : Blocks := []
---   let mut current_and_after : Blocks := freeList
---   while !current_and_after.isEmpty do
---     let (ptr, freeSize) := current_and_after.head!
---     if size <= freeSize then
---       return (before.reverse, current_and_after.head!, current_and_after.tail!)
---     else
---       before := (ptr, freeSize) :: before
---       current_and_after := current_and_after.tail!
---   none -- failure
-
--- def Allocator.alloc (allocator : Allocator) (size: Size) : Option (Pointer × Allocator) := do
---   if size == 0 then
---     return (0, allocator) -- No allocation needed for size 0
---   let (before, current, after) <- findFreeBlock allocator size
---   let (ptr, freeSize) := current
---   let newFreeBlocks := if (size < freeSize) then
---     -- chop the first free block on the left
---     [(ptr + size.toUInt16, freeSize - size)]
---   else
---     [] -- perfect fit, remove the free block entirely
---   let freeList := before ++ newFreeBlocks ++ after
---   let usedList := (ptr, size) :: allocator.usedList
---   return (ptr, { allocator with freeList, usedList })
 
 
 -- Compact contiguous free blocks in allocator.
@@ -166,31 +230,3 @@ partial def Allocator.compact (allocator : Allocator) : Allocator :=
 
 def sortBlocks (blocks : Blocks) : Blocks :=
   blocks.mergeSort (·.1 < ·.1)
-
-partial def Allocator.free (allocator : Allocator) (ptr: Pointer) : Option Allocator := do
-  let freeList := allocator.freeList
-  let usedList := allocator.usedList
-  let block <- usedList.find? (·.1 == ptr)
-  let usedList := usedList.filter (· != block)
-  let freeList := (block :: freeList) |>.mergeSort (·.1 < ·.1)
-  return { allocator with freeList, usedList }.compact
-
-def allocator : Allocator := {}
-
-#eval allocator.alloc 0
-
-#eval allocator.findFreeBlock 1024
-
-#eval allocator.alloc 1024
-
-#eval do
-  let (ptr₁, allocator) <- allocator.alloc 512
-  let (ptr₂, allocator) <- allocator.alloc 512
-  let (_, allocator) <- allocator.alloc 1024
-  let allocator <- allocator.free ptr₁
-  let allocator <- allocator.free ptr₂ -- autocompact
-  return allocator
--- some {
---   freeList := [(0, 512), (512, 512), (2048, 63488)],
---   usedList := [(1024, 1024)]
--- }
